proof/correctness/Utils2.ec
@@ -14,6 +14,14 @@ require import Array8.
 
 (** -------------------------------------------------------------------------------------------- **)
 
+(* from MLKEM proof *)
+op touches (m m' : global_mem_t) (p : address) (len : int) =
+    forall i, !(0 <= i < len) => m'.[p + i] = m.[p + i].
+
+op touches2 (m m' : global_mem_t) (p1 : address) (len1 : int) (p2 : address) (len2 : int) : bool =
+  forall (a : int), ! (p1 <=  a < p1+len1) =>  ! (p2 <=  a < p2+len2) => m'.[a] = m.[a].
+
+
 (* 
   m1 and m2 are memories whose contect is equal except for the indices in the 
   ptr_dif list
@@ -27,6 +35,16 @@ pred mem_dif (m1 m2 : global_mem_t) (ptrs_dif : int list) =
 
 op concatMap  (f: 'a -> 'b list) (a: 'a list): 'b list = flatten (map f a).
 op W32ofBytes (bytes : W8.t list) : W32.t = W32.bits2w (concatMap W8.w2bits bytes).
+op W64ofBytes (bytes : W8.t list) : W64.t = W64.bits2w (concatMap W8.w2bits bytes).
+
+
+lemma W64_W32_of_bytes (t : W8.t list) :
+    0 < size t <= 4 => 
+       to_uint (W32ofBytes t) = to_uint (W64ofBytes t).
+proof.
+move => H.
+admit.
+qed.
 
 (** -------------------------------------------------------------------------------------------- **)
 
@@ -35,6 +53,29 @@ lemma zero_addr_i :
 proof.
 move => k?.
 rewrite /zero_addr initiE // /#.
+qed.
+
+lemma zero_addr_setZero :
+    forall (k : int), 0 <= k < 8 => zero_addr.[k <- W32.zero] = zero_addr.
+proof.
+move => k?.
+rewrite tP => j?.
+rewrite get_setE //.
+case (j = k) => // ?.
+by rewrite zero_addr_i.
+qed.
+
+lemma set_tree_addr_comp (x : W32.t Array8.t) (v1 v2 : int) :
+    set_tree_addr (set_tree_addr x v1) v2 = set_tree_addr x v2.
+proof.
+rewrite /set_tree_addr tP => j?.
+rewrite get_setE //.
+case (j = 2) => *.
+  + by rewrite get_setE // ifT //.
+rewrite get_setE //.
+case (j = 1) => *.
+  + rewrite get_setE // ifF 1:/# get_setE // ifT //.
+by do ! rewrite get_setE // ifF //.
 qed.
 
 (** -------------------------------------------------------------------------------------------- **)
