proof/correctness/VerifyProof.ec
@@ -3,7 +3,7 @@ pragma Goals : printall.
 require import AllCore List RealExp IntDiv Distr DList IntDiv.
 from Jasmin require import JModel JArray.
 
-require import Params Types Address Hash XMSS_MT_Params XMSS_MT_TreeHash XMSS_MT_Types XMSS_MT_PRF.
+require import Params Types Address Hash XMSS_MT_Params WOTS LTree XMSS_MT_TreeHash XMSS_MT_Types XMSS_MT_PRF.
 require import XMSS_IMPL Parameters.
 
 require import Repr2 Utils2.
@@ -11,7 +11,7 @@ require import Repr2 Utils2.
 require import Array4 Array8 Array32 Array64 Array68 Array96 Array132 Array136 Array352 Array2144.
 require import WArray32 WArray96 WArray136.
 
-require import Correctness_Address Correctness_Mem Correctness_Hash.
+require import Correctness_Address Correctness_Bytes Correctness_Mem Correctness_Hash.
 require import DistrUtils.
 
 require import BitEncoding.
@@ -21,6 +21,8 @@ require import StdBigop.
 (*---*) import Bigint.
 
 require import Termination.
+
+require import RootFromSig_Hop.
 
 lemma load_store_W64 (mem : global_mem_t) (a : address) (v : W64.t) :
     loadW64 (storeW64 mem a v) a = v.
@@ -69,15 +71,14 @@ qed.
 lemma p_set_result_post (eq : W8.t) :
     phoare[
       M(Syscall).__set_result :
-      arg.`1 = eq
+      arg.`1 = eq /\
+      0 <= to_uint (loadW64 Glob.mem (to_uint mlen_ptr)) < W64.max_uint
       ==>
       (eq = W8.zero) => res = W64.zero /\
       (eq <> W8.zero) => res = W64.of_int (-1)
     ] = 1%r.
 proof.
-conseq set_result_ll (set_result_post eq).
-  + admit. (* Need to add stuff to #pre *)
-  + admit.
+by conseq set_result_ll (set_result_post eq); auto.
 qed.
 
 (*
@@ -86,7 +87,7 @@ arg{1}
 
 m_ptr : W64.t         => ptr to the message 
 mlen_ptr : W64.t      => ptr to the message length 
-sm_ptr : W64.t        => ptr to the signed message
+sm_ptr : W64.t        => ptr to the signed message ( signed message = signature ++ message )
 smlen : W64.t         => length of the signed message = mlen + sig bytes
 pk : W8.t Array64.t   => public key
 
@@ -97,17 +98,9 @@ m : msg_t     => message
 s : sig_t    => signature How to encode signature ?
 *)
 
-(* Load the signed message from memory. res = m || sig *)
-op load_sm_mem (mem : global_mem_t) (ptr sm_len : W64.t) : W8.t list =
-    mkseq (fun (i : int) => loadW8 mem (to_uint ptr + i)) (to_uint sm_len).
-
-(* Load the signature from memory. Skips the message *)
+(* Load the signature from memory. Ignores the message *)
 op load_sig_mem (mem : global_mem_t) (sm_ptr sm_len : W64.t) : W8.t list =
-    let mlen : int = to_uint sm_len - XMSS_SIG_BYTES in
-    mkseq (fun (i : int) => loadW8 mem (to_uint sm_ptr + mlen + i)) XMSS_SIG_BYTES.
-
-print EncodeSignature. (* byte list -> sig_t *)
-print load_signature_mem. (* ptr & len  -> byte list *)
+    mkseq (fun (i : int) => loadW8 mem (to_uint sm_ptr + i)) XMSS_SIG_BYTES.
 
 lemma verify_correctness (mem : global_mem_t)  (ptr_m ptr_mlen ptr_sm sm_len : W64.t) (_pk : W8.t Array64.t) :
     n = XMSS_N /\
@@ -119,27 +112,47 @@ lemma verify_correctness (mem : global_mem_t)  (ptr_m ptr_mlen ptr_sm sm_len : W
       Glob.mem{1} = mem /\
 
       0 < to_uint (loadW64 mem (to_uint ptr_mlen)) < W64.max_uint /\
-      valid_ptr_i ptr_sm (4 + 32) /\
+      valid_ptr_i ptr_sm 36 /\
+      valid_ptr_i ptr_m 2372 /\
+
+      XMSS_SIG_BYTES < to_uint sm_len /\
 
       arg{1} = (ptr_m, ptr_mlen, ptr_sm, sm_len, _pk) /\
       arg{2}.`1 = EncodePkNoOID _pk /\
       arg{2}.`2 = load_sig_mem mem ptr_sm sm_len /\
       arg{2}.`3 = EncodeSignature ( load_signature_mem mem ptr_sm (sm_len - W64.of_int XMSS_SIG_BYTES) )
       ==>
-      res{2}  <=> res{1} = W64.zero /\
-      (!res{2} <=> res{1} = W64.of_int (-1))
+      (res{2} <=> res{1} = W64.zero) 
     ].
 proof.
 rewrite /XMSS_N /XMSS_D /XMSS_FULL_HEIGHT => [#] n_val d_val h_val.
 proc => /=. 
 seq 9 0 : #pre; first by auto.
-seq 29 17 : (is_valid{2} <=> are_equal{1} = W8.zero); last first.
+(*
+seq 29 17 : (
+  (0 <= to_uint (loadW64 Glob.mem{1} (to_uint mlen_ptr{1})) < W64.max_uint) /\
+  is_valid{2} <=> are_equal{1} = W8.zero
+); last first.
   + ecall {1} (p_set_result_post are_equal{1}).
-    auto => /> &1 r *.
-    case (are_equal{1} = W8.zero) => *.
-       - admit.
-       - admit.
-        
+    auto => /> &1 &2. 
+    move => [H H1]. 
+ do split.
+    have E : (0 <= to_uint (loadW64 Glob.mem{1} (to_uint mlen_ptr{1})) &&
+    to_uint (loadW64 Glob.mem{1} (to_uint mlen_ptr{1})) <
+    18446744073709551615)
+
+
+
+       * smt(@W64 pow2_64). 
+       * move => ?.  
+         admit. (* This is in H *)
+       * move => ?? r *; do split.         
+            - admit.
+            - admit.
+            - admit.
+            - admit.
+*)
+
 seq 3 0 : (
   #pre /\
   sm_offset{1} = W64.zero /\
@@ -202,7 +215,10 @@ seq 4 0 : (
 conseq (:
     Glob.mem{1} = mem /\
     (0 < to_uint (loadW64 mem (to_uint ptr_mlen)) < W64.max_uint) /\
-    valid_ptr_i ptr_sm 36 /\
+
+      valid_ptr_i ptr_sm 36 /\
+      valid_ptr_i ptr_m 2372 /\
+
     m_ptr{1} = ptr_m /\
     mlen_ptr{1} = ptr_mlen /\
     sm_ptr{1} = ptr_sm /\ 
@@ -218,7 +234,9 @@ conseq (:
 
     ots_addr{1} = zero_address /\
     ltree_addr{1} = zero_address.[3 <- W32.one] /\
-    node_addr{1} = zero_address.[3 <- W32.of_int 2]
+    node_addr{1} = zero_address.[3 <- W32.of_int 2] /\
+
+         XMSS_SIG_BYTES < to_uint sm_len
 
     ==>
     _
@@ -233,12 +251,13 @@ conseq (:
            rewrite get_setE // initiE //.
            case (j = 3) => /#. 
 
-(* This corresponds to *mlen = smlen - params->sig_bytes;
-   Not useful for the proof but #pre no longer holds 
-*)
+(* This corresponds to *mlen = smlen - params->sig_bytes; *)
 seq 3 0 : (
   (0 < to_uint (loadW64 mem (to_uint ptr_mlen))  < W64.max_uint) /\
-  valid_ptr_i ptr_sm 36 /\
+
+    valid_ptr_i ptr_sm 36 /\
+      valid_ptr_i ptr_m 2372 /\
+
   m_ptr{1} = ptr_m /\
   mlen_ptr{1} = ptr_mlen /\
   sm_ptr{1} = ptr_sm /\
@@ -253,8 +272,14 @@ seq 3 0 : (
   to_list pub_seed{1} = sub pk{1} 32 32 /\
   ots_addr{1} = zero_address /\
   ltree_addr{1} = zero_address.[3 <- W32.one] /\
-  node_addr{1} = zero_address.[3 <- (of_int 2)%W32]
-); first by auto.
+  node_addr{1} = zero_address.[3 <- (of_int 2)%W32] /\
+
+
+  loadW64 Glob.mem{1} (to_uint mlen_ptr{1}) = smlen{1} - (W64.of_int 2500) /\
+      XMSS_SIG_BYTES < to_uint sm_len{1}
+).
+    + auto => /> &1 *.
+      by rewrite load_store_W64.
 
 seq 1 2 : (
   #pre /\ 
@@ -262,7 +287,38 @@ seq 1 2 : (
   idx_sig{2} = s{2}.`sig_idx
 ).
     + auto => />.
-      admit. 
+      ecall {1} (bytes_to_ull_ptr_correct Glob.mem{1} sm_ptr{1}).
+      auto => /> &1 *; split; first by smt(@W64 pow2_64).
+      move => *.
+      rewrite /EncodeSignature => />.
+      rewrite W64_W32_of_bytes; [ by rewrite size_sub_list |].  
+      congr. 
+      rewrite wordP => j?.
+      rewrite /W64ofBytes /bits2w !initiE // => />.
+      rewrite /concatMap.
+      (* a partir daqui esta mal *)
+      rewrite !(nth_flatten false 8).
+          * pose P := (fun (s : bool list) => size s = 8).
+            pose L := (map W8.w2bits (mkseq (fun (i0 : int) => loadW8 Glob.mem{1} (to_uint ptr_sm + i0)) 4)).
+            rewrite -(all_nthP P L witness) /P /L size_map size_mkseq (: max 0 4 = 4) // => i?. 
+            rewrite (nth_map witness); first by rewrite size_mkseq //.
+            rewrite /w2bits size_mkseq //.
+          * pose P := (fun (s : bool list) => size s = 8).
+            pose L := (map W8.w2bits (sub_list (load_signature_mem mem ptr_sm (sm_len - (of_int XMSS_SIG_BYTES)%W64)) 0 4)).
+            rewrite -(all_nthP P L witness) /P /L size_map size_mkseq (: max 0 4 = 4) // => i?. 
+            rewrite (nth_map witness); first by rewrite size_mkseq //.
+            rewrite /w2bits size_mkseq //.
+      rewrite !(nth_map witness). 
+          * rewrite size_mkseq. admit.
+          * rewrite size_iota. admit.
+          * rewrite size_sub_list //. admit.
+          * rewrite size_iota. admit.
+      rewrite /w2bits nth_mkseq 1:/# nth_mkseq 1:/# => />.
+      rewrite /load_signature_mem nth_mkseq nth_iota.
+          * admit.
+          * smt(). 
+          * admit.
+      admit.
 
 (* This corresponds to the comment 
 
@@ -271,23 +327,22 @@ seq 1 2 : (
     
     This is not useful for the proof 
 *)
-seq 4 0 : (#pre).
+seq 4 0 : (#pre). 
     + seq 3 0 : (#pre /\ 0 <= to_uint bytes{1} < W64.max_uint).
-         * auto => /> &1 *; split. 
-              - admit.
-              - admit. (* A partir de #pre nao sei que Glob.mem.[ptr_m] = mem.[ptr_m] *)
-
+         * auto => /> &1 ???????? -> *; split => [| ?]. 
+              - smt(@W64 pow2_64).
+              - rewrite to_uintB; [by rewrite uleE of_uintK /= /# |]. 
+                rewrite of_uintK /= #smt:(@W64 pow2_64).
       inline {1}.
-      while {1} (#post) (to_uint bytes2{1} - to_uint i0{1}).
-         * auto => /> &hr *; smt(@W64 pow2_64).
-         * auto => /> &1 *; rewrite ultE /#.
+      while {1} (#post) (to_uint bytes2{1} - to_uint i0{1}); last by auto => /> *; rewrite ultE /#.
+      admit.
   
 seq 0 2 : (
     #pre /\
     val seed{2} = to_list pub_seed{1} /\
     address{2} = zero_address
 ).
-    + auto => /> &1 &2 ???? -> *. 
+    + auto => /> &1 &2 ?????? -> *. 
       (* A seta refere se a hipotese to_list pub_seed{1} = sub _pk 32 32 *)
       apply (eq_from_nth witness); first by rewrite valP n_val size_sub.
       rewrite valP n_val => j?.
@@ -312,7 +367,11 @@ seq 3 0 : (
 
 swap {2} 5 -4.
 seq 0 1 : (#pre /\ to_list buf{1} = val _R{2}).
-    + auto => /> &1 &2 ???????? ->. 
+    + auto => /> &1 &2 ???????????? ->. 
+(* A seta refere se a hipotese to_list buf{1} =
+   mkseq (fun (i0 : int) => loadW8 Glob.mem{1} (to_uint ptr_sm + 4 + i0)) 32
+*)
+
       apply (eq_from_nth witness).
          * by rewrite valP n_val size_mkseq.
       rewrite size_mkseq => j?.
@@ -323,15 +382,17 @@ seq 0 1 : (#pre /\ to_list buf{1} = val _R{2}).
       rewrite to_uintD.
       admit.
 
-
 seq 3 0  : (
   #pre /\
   to_uint t64{1} = to_uint m_ptr{1} + 2500 - 32 - 3*32 /\
   to_uint bytes{1} = to_uint smlen{1} - XMSS_SIG_BYTES
 ).
-    + auto => /> &1 &2 *; split.
-        * rewrite to_uintD of_uintK /=.  admit. (* Add info to precondition *)
-        * admit. (* Not enough info => Adicionar aquela parte que passei a frente *)
+    + auto => /> &1 &2 ???????? -> *; split.
+(* A seta refere se a hipotese loadW64 Glob.mem{1} (to_uint ptr_mlen) = sm_len - (of_int 2500)%W64 *)
+        * rewrite to_uintD of_uintK /= /#. 
+        * rewrite /XMSS_SIG_BYTES to_uintB.
+             - rewrite uleE of_uintK /= /#.
+          rewrite of_uintK /#.
 
 seq 0 2 : (
   #pre /\
@@ -353,10 +414,11 @@ swap {2} 1 4.
 seq 1 2 : (#pre /\ to_list root{1} = val _M'{2}).
     + admit.
 
-
-seq 0 2 : (
+(* #pre but update sm_offset *) 
+seq 2 1 : (
   0 < to_uint (loadW64 mem (to_uint ptr_mlen)) < W64.max_uint /\
   valid_ptr_i ptr_sm 36 /\
+  valid_ptr_i ptr_m 2372 /\
   m_ptr{1} = ptr_m /\
   mlen_ptr{1} = ptr_mlen /\
   sm_ptr{1} = ptr_sm /\
@@ -364,42 +426,41 @@ seq 0 2 : (
   pk{1} = _pk /\
   pk{2} = EncodePkNoOID _pk /\
   m{2} = load_sig_mem mem ptr_sm sm_len /\
-  s{2} =
-    EncodeSignature (load_signature_mem mem ptr_sm  (sm_len - (of_int XMSS_SIG_BYTES)%W64)) /\
-  sm_offset{1} = W64.zero /\
+  s{2} = EncodeSignature (load_signature_mem mem ptr_sm (sm_len - (of_int XMSS_SIG_BYTES)%W64)) /\
   to_list pub_root{1} = sub pk{1} 0 32 /\
   to_list pub_seed{1} = sub pk{1} 32 32 /\
   ots_addr{1} = zero_address /\
   ltree_addr{1} = zero_address.[3 <- W32.one] /\
   node_addr{1} = zero_address.[3 <- (of_int 2)%W32] /\
-  to_uint idx{1} = to_uint idx_sig{2} /\ idx_sig{2} = s{2}.`sig_idx /\
-  val seed{2} = to_list pub_seed{1}  /\
-  to_list buf{1} =
-    mkseq (fun (i0 : int) => loadW8 Glob.mem{1} (to_uint sm_ptr{1} + 4 + i0)) 32 /\
+  loadW64 Glob.mem{1} (to_uint mlen_ptr{1}) = smlen{1} - (of_int 2500)%W64 /\ 
+  XMSS_SIG_BYTES < to_uint sm_len /\ 
+  to_uint idx{1} = to_uint idx_sig{2} /\ 
+  idx_sig{2} = s{2}.`sig_idx /\
+  val seed{2} = to_list pub_seed{1} /\
+  address{2} = zero_address /\
+  to_list buf{1} = mkseq (fun (i0 : int) => loadW8 Glob.mem{1} (to_uint sm_ptr{1} + 4 + i0)) 32 /\
   to_list buf{1} = val _R{2} /\
   to_uint bytes{1} = to_uint smlen{1} - XMSS_SIG_BYTES /\
   idx_tree{2} = idx_sig{2} `>>>` 10 /\
   idx_leaf{2} = idx_sig{2} `&` (of_int (2 ^ 10 - 1))%W32 /\
   val root{2} = sub pk{1} 0 32 /\
   to_list root{1} = val _M'{2} /\
-  
-  
-  address{2} = zero_address.[1 <- idx_tree{2}]
+
+  to_uint sm_offset{1} = 4 + 32
 ).
     + auto => /> &1 &2 *.
-      rewrite /set_tree_addr /set_layer_addr.
-      rewrite tP => j?.
-      case (j = 0) => *. 
-         * by rewrite get_setE // ifF 1:/# get_setE // ifF 1:/# get_setE // ifT // get_setE // ifF 1:/# zero_addr_i.
-      case (j = 1) => *.
-         * rewrite get_setE // ifF 1:/# get_setE // ifT // get_setE // ifT //.
-           admit.
-     admit.
+      rewrite /set_layer_addr /zero_address tP => j?.
+      rewrite get_setE // .
+      case (j = 0) => [? | //]. 
+      by rewrite initiE.
+
+(* #pre but update address{2} *)
 
 
-seq 2 0 : (
+seq 0 1 : (
   0 < to_uint (loadW64 mem (to_uint ptr_mlen)) < W64.max_uint /\
   valid_ptr_i ptr_sm 36 /\
+  valid_ptr_i ptr_m 2372 /\
   m_ptr{1} = ptr_m /\
   mlen_ptr{1} = ptr_mlen /\
   sm_ptr{1} = ptr_sm /\
@@ -407,75 +468,104 @@ seq 2 0 : (
   pk{1} = _pk /\
   pk{2} = EncodePkNoOID _pk /\
   m{2} = load_sig_mem mem ptr_sm sm_len /\
-  s{2} =
-    EncodeSignature (load_signature_mem mem ptr_sm  (sm_len - (of_int XMSS_SIG_BYTES)%W64)) /\
+  s{2} = EncodeSignature (load_signature_mem mem ptr_sm (sm_len - (of_int XMSS_SIG_BYTES)%W64)) /\
   to_list pub_root{1} = sub pk{1} 0 32 /\
   to_list pub_seed{1} = sub pk{1} 32 32 /\
   ots_addr{1} = zero_address /\
   ltree_addr{1} = zero_address.[3 <- W32.one] /\
   node_addr{1} = zero_address.[3 <- (of_int 2)%W32] /\
-  to_uint idx{1} = to_uint idx_sig{2} /\ idx_sig{2} = s{2}.`sig_idx /\
-  val seed{2} = to_list pub_seed{1}  /\
-  to_list buf{1} =
-    mkseq (fun (i0 : int) => loadW8 Glob.mem{1} (to_uint sm_ptr{1} + 4 + i0)) 32 /\
+  loadW64 Glob.mem{1} (to_uint mlen_ptr{1}) = smlen{1} - (of_int 2500)%W64 /\ 
+  XMSS_SIG_BYTES < to_uint sm_len /\ 
+  to_uint idx{1} = to_uint idx_sig{2} /\ 
+  idx_sig{2} = s{2}.`sig_idx /\
+  val seed{2} = to_list pub_seed{1} /\
+  to_list buf{1} = mkseq (fun (i0 : int) => loadW8 Glob.mem{1} (to_uint sm_ptr{1} + 4 + i0)) 32 /\
   to_list buf{1} = val _R{2} /\
   to_uint bytes{1} = to_uint smlen{1} - XMSS_SIG_BYTES /\
   idx_tree{2} = idx_sig{2} `>>>` 10 /\
   idx_leaf{2} = idx_sig{2} `&` (of_int (2 ^ 10 - 1))%W32 /\
   val root{2} = sub pk{1} 0 32 /\
   to_list root{1} = val _M'{2} /\
-  
-  
-  address{2} = zero_address.[1 <- idx_tree{2}] /\
 
-  to_uint t64{1} = 36 /\ 
-  to_uint sm_offset{1} = 36
+  to_uint sm_offset{1} = 4 + 32 /\
+
+  address{2} = set_tree_addr zero_address (to_uint (s{2}.`sig_idx `>>>` 10))
+); first by auto.  
+
+unroll {1} 2.
+rcondt {1} 2; first by auto.
+print truncateu32.
+seq 3 0 : (
+  #pre /\
+  i{1} = W32.zero /\
+  idx_leaf{1} = (of_int (2^10 - 1))%W32 `&` (truncateu32 idx{1})
 ); first by auto.
 
+swap{1} 3.
 
-(* Unroll the first iteration on the left hand side *)
-unroll {1} 2.
+seq 3 0 : (#pre).
+    + inline {1}; auto => /> *.
+      do split.
+          * by apply zero_addr_setZero.
+          * rewrite tP => j?.
+            rewrite get_setE //.
+            case (j = 0) => ?; last by rewrite get_setE.
+            by rewrite get_setE // ifF 1:/# zero_addr_i.
+          * rewrite tP => j?.
+            rewrite get_setE //.
+            case (j = 0) => ?; last by rewrite get_setE.
+            by rewrite get_setE // ifF 1:/# zero_addr_i.
+          
+(** ------------------------------------------------------------------------------------------------------------------------------------------------ **)
 
-(* inline {2} RootFromSig.rootFromSig. *)
-(* Outline the inner loop *)
-(* cf. https://github.com/EasyCrypt/easycrypt/wiki/%5BTactic%5D-Outline *)
+seq 24 4 : (
+0 <= to_uint (loadW64 Glob.mem{1} (to_uint mlen_ptr{1})) < W64.max_uint /\
+val node{2} = to_list root{1} /\
+val root{2} = to_list pub_root{1} /\
+is_valid{2} = (are_equal{1} = W8.zero)
+); last first.
 
-rcondt {1} 2; first by auto.
+    + case (root{1} = pub_root{1}).
+         * seq 1 0 : (val node{2} = to_list root{1} /\
+                      val root{2} = to_list pub_root{1} /\
+                      root{1} = pub_root{1} /\ 
+                      0 <= to_uint (loadW64 Glob.mem{1} (to_uint mlen_ptr{1})) < W64.max_uint /\ 
+                      are_equal{1} = W8.zero).
+               - exists * root{1}, pub_root{1}.
+                 elim * => P0 P1.
+                 call {1} (p_memcmp_true P0 P1); last by auto.
+                 admit. (* Nao percebi => Quando chego a este subgoal ja nao ha informacao sobre P0 e P1 *)     
+           ecall {1} (p_set_result_post are_equal{1}).
+           auto => /> &1 &2 H0 H1 *.
+           do split.
+               - admit.
+               - apply nbytes_eq. 
+                 by rewrite H0 H1.
 
-seq 2 0 : (#pre /\ to_uint idx_leaf{1} = 2^10 - 1); first by auto.
+         * seq 1 0 : (val node{2} = to_list root{1} /\
+                      val root{2} = to_list pub_root{1} /\
+                      root{1} <> pub_root{1} /\ 
+                      0 <= to_uint (loadW64 Glob.mem{1} (to_uint mlen_ptr{1})) < W64.max_uint /\ are_equal{1} 
+                      <> W8.zero).
+               - exists * root{1}, pub_root{1}.
+                 elim * => P0 P1.
+                 call {1} (p_memcmp_false P0 P1); last by auto.
+                 admit. (* Nao percebi => Quando chego a este subgoal ja nao ha informacao sobre P0 e P1 *)     
+           ecall {1} (p_set_result_post are_equal{1}).
+           auto => /> &1 &2 H0 H1*.
+           do split => [* |].
+               - admit.
+               - apply nbytes_eq. 
+                 rewrite H0 H1.
+                 admit. (* This is false *)
 
+(** ------------------------------------------------------------------------------------------------------------------------------------------------ **)
 
-qed.
-
-
-
-(*
-(* We have that sub sm_ptr 0 4 = W32ofBytes x.sig_idx => TODO: I need to write this lemma *)
-    + admit.
-
-
-swap {2} [2..3] -1.
-seq 0 2 : (#pre /\ to_list pub_seed{1} = val seed{2}).
-    + auto => /> &1 &2 ???? H*.
-      apply (eq_from_nth witness); first by rewrite valP n_val size_to_list.
-      rewrite size_to_list => j?.
-      rewrite /EncodePkNoOID => />. 
-      rewrite insubdK; first by rewrite /P size_sub // n_val. 
-      by rewrite -get_to_list H.
-
-(* This corresponds to memcpy(m + params->sig_bytes, sm + params->sig_bytes, *mlen)
-   Lines  452 - 456 in the xmss_commons.jtmpl 
-*)
-seq 4 0 : (#pre).  (* this is irrelevant for the result of the proof => just stores *)
-    + admit.
-
-
-(* this conseq simplifies #pre so it fits on the screen *)
-conseq (:
-    Glob.mem{2} = mem /\
-  (0 < to_uint (loadW64 Glob.mem{1} (to_uint ptr_mlen))  < W64.max_uint) /\
-    mem_dif Glob.mem{1} Glob.mem{2} [to_uint mlen_ptr{1}] /\
-    t64{1} = smlen{1} - (of_int XMSS_SIG_BYTES)%W64 /\
+(* Replaced truncateu32 idx{1} with idx_sig{2} *)
+seq 1 0 : (
+    0 < to_uint (loadW64 mem (to_uint ptr_mlen)) < W64.max_uint /\
+    valid_ptr_i ptr_sm 36 /\
+    valid_ptr_i ptr_m 2372 /\
     m_ptr{1} = ptr_m /\
     mlen_ptr{1} = ptr_mlen /\
     sm_ptr{1} = ptr_sm /\
@@ -483,41 +573,200 @@ conseq (:
     pk{1} = _pk /\
     pk{2} = EncodePkNoOID _pk /\
     m{2} = load_sig_mem mem ptr_sm sm_len /\
-    s{2} = witness /\
-    sm_offset{1} = W64.zero /\
+    s{2} = EncodeSignature (load_signature_mem mem ptr_sm (sm_len - (of_int XMSS_SIG_BYTES)%W64)) /\
     to_list pub_root{1} = sub pk{1} 0 32 /\
     to_list pub_seed{1} = sub pk{1} 32 32 /\
-    
     ots_addr{1} = zero_address /\
     ltree_addr{1} = zero_address.[3 <- W32.one] /\
-    node_addr{1} = zero_address.[3 <- W32.of_int 2]
+    node_addr{1} = zero_address.[3 <- (of_int 2)%W32] /\
+    loadW64 Glob.mem{1} (to_uint mlen_ptr{1}) = smlen{1} - (of_int 2500)%W64 /\
+    XMSS_SIG_BYTES < to_uint sm_len /\
+    idx_sig{2} = s{2}.`sig_idx /\
+    val seed{2} = to_list pub_seed{1} /\
+    to_list buf{1} = mkseq (fun (i0 : int) => loadW8 Glob.mem{1} (to_uint sm_ptr{1} + 4 + i0)) 32 /\
+    to_list buf{1} = val _R{2} /\
+    to_uint bytes{1} = to_uint smlen{1} - XMSS_SIG_BYTES /\
+    idx_tree{2} = idx_sig{2} `>>>` 10 /\
+    idx_leaf{2} = idx_sig{2} `&` (of_int (2 ^ 10 - 1))%W32 /\
+    val root{2} = sub pk{1} 0 32 /\
+    to_list root{1} = val _M'{2} /\
+    to_uint sm_offset{1} = 4 + 32 /\
+    address{2} = set_tree_addr zero_address (to_uint (s{2}.`sig_idx `>>>` 10)) /\
+    i{1} = W32.zero /\
+    idx_leaf{1} = (of_int (2 ^ 10 - 1))%W32 `&` idx_sig{2} /\
+
+
+    (* neste shift substitui idx{1} : W64.t por zeroextu64 idx_sig{2} *)  
+    idx{1} = zeroextu64 idx_sig{2} `>>` truncateu8 (W256.of_int 10 `&` W256.of_int 63)
+).
+    + auto => /> &1 &2 *; split.
+         * congr.
+           rewrite /EncodeSignature /load_signature_mem => />.
+           rewrite wordP => j?.
+           admit.
+         * congr.  
+           rewrite /EncodeSignature /load_signature_mem => />.
+           rewrite wordP => j?.
+           admit.
+
+seq 4 0 : (
+    0 < to_uint (loadW64 mem (to_uint ptr_mlen)) < W64.max_uint /\
+    valid_ptr_i ptr_sm 36 /\
+    valid_ptr_i ptr_m 2372 /\
+    m_ptr{1} = ptr_m /\
+    mlen_ptr{1} = ptr_mlen /\
+    sm_ptr{1} = ptr_sm /\
+    smlen{1} = sm_len /\
+    pk{1} = _pk /\
+    pk{2} = EncodePkNoOID _pk /\
+    m{2} = load_sig_mem mem ptr_sm sm_len /\
+    s{2} = EncodeSignature (load_signature_mem mem ptr_sm (sm_len - (of_int XMSS_SIG_BYTES)%W64)) /\
+    to_list pub_root{1} = sub pk{1} 0 32 /\
+    to_list pub_seed{1} = sub pk{1} 32 32 /\
+    loadW64 Glob.mem{1} (to_uint mlen_ptr{1}) = smlen{1} - (of_int 2500)%W64 /\
+    XMSS_SIG_BYTES < to_uint sm_len /\
+    idx_sig{2} = s{2}.`sig_idx /\
+    val seed{2} = to_list pub_seed{1} /\
+    to_list buf{1} = mkseq (fun (i0 : int) => loadW8 Glob.mem{1} (to_uint sm_ptr{1} + 4 + i0)) 32 /\
+    to_list buf{1} = val _R{2} /\
+    to_uint bytes{1} = to_uint smlen{1} - XMSS_SIG_BYTES /\
+    idx_tree{2} = idx_sig{2} `>>>` 10 /\
+    idx_leaf{2} = idx_sig{2} `&` (of_int (2 ^ 10 - 1))%W32 /\
+    val root{2} = sub pk{1} 0 32 /\
+    to_list root{1} = val _M'{2} /\
+    to_uint sm_offset{1} = 4 + 32 /\
+    address{2} = set_tree_addr zero_address (to_uint (s{2}.`sig_idx `>>>` 10)) /\
+    i{1} = W32.zero /\
+    idx_leaf{1} = (of_int (2 ^ 10 - 1))%W32 `&` idx_sig{2} /\
+
+    idx{1} = zeroextu64 idx_sig{2} `>>` truncateu8 (W256.of_int 10 `&` W256.of_int 63) /\
+
+    ots_addr{1} = set_tree_addr (set_tree_addr zero_address (to_uint idx{1})) (to_uint idx_leaf{1}) /\
+    ltree_addr{1} = set_tree_addr (zero_address.[3 <- W32.one]) (to_uint idx{1}) /\
+    node_addr{1} = set_tree_addr (zero_address.[3 <- (of_int 2)%W32]) (to_uint idx{1})
+).
+    + inline {1}.
+      auto => /> &1 &2 *.
+      admit.
+
+
+conseq (:
+    0 < to_uint (loadW64 mem (to_uint ptr_mlen)) < W64.max_uint /\
+    valid_ptr_i ptr_sm 36 /\
+    valid_ptr_i ptr_m 2372 /\
+    m_ptr{1} = ptr_m /\
+    mlen_ptr{1} = ptr_mlen /\
+    sm_ptr{1} = ptr_sm /\
+    smlen{1} = sm_len /\
+    pk{1} = _pk /\
+    pk{2} = EncodePkNoOID _pk /\
+    m{2} = load_sig_mem mem ptr_sm sm_len /\
+    s{2} = EncodeSignature (load_signature_mem mem ptr_sm (sm_len - (of_int XMSS_SIG_BYTES)%W64)) /\
+    to_list pub_root{1} = sub pk{1} 0 32 /\
+    to_list pub_seed{1} = sub pk{1} 32 32 /\
+    loadW64 Glob.mem{1} (to_uint mlen_ptr{1}) = smlen{1} - (of_int 2500)%W64 /\
+    XMSS_SIG_BYTES < to_uint sm_len /\
+    idx_sig{2} = s{2}.`sig_idx /\
+    val seed{2} = to_list pub_seed{1} /\
+    to_list buf{1} = mkseq (fun (i0 : int) => loadW8 Glob.mem{1} (to_uint sm_ptr{1} + 4 + i0)) 32 /\
+    to_list buf{1} = val _R{2} /\
+    to_uint bytes{1} = to_uint smlen{1} - XMSS_SIG_BYTES /\
+    idx_tree{2} = idx_sig{2} `>>>` 10 /\
+    idx_leaf{2} = idx_sig{2} `&` (of_int (2 ^ 10 - 1))%W32 /\
+    val root{2} = sub pk{1} 0 32 /\
+    to_list root{1} = val _M'{2} /\
+    to_uint sm_offset{1} = 4 + 32 /\
+    address{2} = set_tree_addr zero_address (to_uint (s{2}.`sig_idx `>>>` 10)) /\
+    i{1} = W32.zero /\
+    idx_leaf{1} = (of_int (2 ^ 10 - 1))%W32 `&` idx_sig{2} /\
+
+    idx{1} = zeroextu64 idx_sig{2} `>>` truncateu8 (W256.of_int 10 `&` W256.of_int 63) /\
+
+    (* This was simplified using lemma set_tree_addr_comp *)
+    ots_addr{1} = set_tree_addr zero_address (to_uint idx_leaf{1}) /\
+    ltree_addr{1} = set_tree_addr (zero_address.[3 <- W32.one]) (to_uint idx{1}) /\
+    node_addr{1} = set_tree_addr (zero_address.[3 <- (of_int 2)%W32]) (to_uint idx{1})
+
   ==>
   _
 ).
-    + auto => /> &1 &2 *; do split.
-         * rewrite /zero_address tP => j?.
-           rewrite initiE // /#.
-         * rewrite /zero_address tP => j?.
-           rewrite get_setE // initiE //.
-           case (j = 3) => /#. 
-         * rewrite /zero_address tP => j?.
-           rewrite get_setE // initiE //.
-           case (j = 3) => /#. 
+    + auto => /> &1 &2 *.
+      rewrite set_tree_addr_comp //.
 
-(* This corresponds to the comment 
-1) First we need to copy the randomness from sm + params->index_bytes to buf
-*)
-swap {2} 6 -5.
-seq 3 1 : (
-  #pre /\ 
-  to_list buf{1} = val _R{2}
+seq 2 1 : (
+  #pre /\
+  t64{1} = sm_ptr{1} + sm_offset{1} /\
+  (sig_ots{2}, auth{2}) = nth witness s{2}.`r_sigs 0
+); first by auto => /> /#.
+
+inline {2} 1.
+
+seq 1 0 : #pre; first by auto.
+
+
+seq 0 6 : (
+  #pre /\
+  idx_sig0{2} = idx_leaf{2} /\                           
+  sig_ots0{2} = sig_ots{2} /\
+  auth0{2} = auth{2} /\
+  M{2} = _M'{2} /\                             
+  _seed{2} = seed{2} /\
+  address0{2} = address{2}
+);first by auto.
+
+seq 0 2 : (
+    #{/~address0{2} = address{2}}pre /\
+  address0{2} = set_ots_addr (set_tree_addr zero_address (to_uint (s{2}.`sig_idx `>>>` 10))) (to_uint idx_sig{2})
+).
+    + auto => /> &1 &2 *.
+      rewrite tP => j?.
+      do 2! congr; last first.
+        * admit.
+      rewrite /set_type /set_tree_addr.
+      admit.
+
+
+
+
+
+
+
+(* #pre no longer holds : the value of root was changed *)
+seq 1 1 : (
+    #{/~to_list root{1} = val _M'{2}}
+     {/~ots_addr{1} = set_tree_addr zero_address (to_uint idx_leaf{1})}pre /\
+      wots_pk{1} = DecodeWotsPk pk_ots{2}
+(*     ots_addr{1}.[0-4]   ====> cf. Properties Address *)
 ).
     + admit.
+  
 
-(* Unroll the first iteration on the left hand side *)
-unroll {1} 9.
+seq 2 0 : (
+  #{/~t64{1} = sm_ptr{1} + sm_offset{1}}pre /\
+  to_uint t64{1} = 2180 
+). 
+    + auto => /> &1 &2 ??????????????? H?.
+      rewrite to_uintD_small; [by rewrite H of_uintK |].
+      by rewrite H of_uintK /=.
+seq 1 0 : (#{/~to_uint sm_offset{1} = 4 + 32}pre /\ sm_offset{1} = t64{1}); first by auto.
 
+(* Not sure if #pre is preserved *)
+seq 2 3 : (#pre /\ to_list leaf{1} = val nodes0{2}).
+    + admit.
 
-admit.
-qed.
-*)
+(* https://github.com/EasyCrypt/easycrypt/wiki/%5BTactic%5D-Outline *)
+outline {2} [3-4] (node) <@ RootFromSig_Hop.rootFromSigInnerLoop; last first.    (* So quero substituir isto do lado direito *)
+                                                                                 (* Nao percebi pq esta a gerar um subgoal com a substituicao feita do lado esquedo ? *)
+    + admit.
+ 
+seq 4 0 : (
+    #{/~to_uint t64{1} = 2180}
+     {/~sm_offset{1} = t64{1}}pre  /\
+    t64{1} = sm_ptr{1} + W64.of_int 2180 /\
+    sm_offset{1} = W64.of_int 2180
+); first by auto => /> *; split; smt(@W64 pow2_64).
+
+seq 1 3 : (
+  #pre
+).
+
